removing an admit from the unionfind example, took much longer than expected, needed to completely change the forest invariants

examples/dm4free/Relational.UnionFind.fst
@@ -1,131 +1,160 @@
 module Relational.UnionFind
 
 open FStar.Seq
+open FStar.OrdSet
+
 open FStar.DM4F.Heap
 open FStar.DM4F.Heap.ST
 
+type subtree_t = ordset nat (fun x y -> x <= y)
+
+(***** some boring set lemmas *****)
+assume val minus: subtree_t -> subtree_t -> Tot subtree_t
+assume val strict_subset: subtree_t -> subtree_t -> Tot bool
+assume val set_n (n:nat): subtree_t
+
+let lemma_strict_subset_size (s1:subtree_t) (s2:subtree_t)
+  :Lemma (requires (strict_subset s1 s2))
+         (ensures  (subset s1 s2 /\ size s1 < size s2))
+   [SMTPat (strict_subset s1 s2)]
+  = admit ()
+
+let lemma_minus_mem (s1:subtree_t) (s2:subtree_t) (x:nat)
+  :Lemma (requires True) (ensures (mem x (minus s1 s2) = (mem x s1 && not (mem x s2))))
+   [SMTPat (mem x (minus s1 s2))]
+  = admit ()
+
+let lemma_strict_subset_minus_size (s:subtree_t) (s1:subtree_t) (s2:subtree_t)
+  :Lemma (requires (strict_subset s1 s2 /\ subset s1 s /\ subset s2 s))
+         (ensures  (size (minus s s2) < size (minus s s1)))
+   [SMTPat (strict_subset s1 s2); SMTPat (subset s1 s); SMTPat (subset s2 s)]
+  = admit ()
+
+let lemma_disjoint_union_subset (s1:subtree_t) (s2:subtree_t)
+  :Lemma (requires (~ (s1 == empty) /\ ~ (s2 == empty) /\ intersect s1 s2 == empty))
+         (ensures  (strict_subset s1 (union s1 s2) /\ strict_subset s2 (union s1 s2)))
+   [SMTPatOr [[SMTPat (strict_subset s1 (union s1 s2))]; [SMTPat (strict_subset s2 (union s1 s2))]]]
+  = admit ()
+
+let lemma_subset_union (s1:subtree_t) (s2:subtree_t) (n:nat)
+  :Lemma (requires (subset s1 (set_n n) /\ subset s2 (set_n n)))
+         (ensures  (subset (union s1 s2) (set_n n)))
+   [SMTPat (subset (union s1 s2) (set_n n))]
+  = ()
+
+let lemma_strict_subset_transitive (s1:subtree_t) (s2:subtree_t) (s3:subtree_t)
+  :Lemma (requires (strict_subset s1 s2 /\ strict_subset s2 s3))
+         (ensures  (strict_subset s1 s3))
+   [SMTPat (strict_subset s1 s2); SMTPat (strict_subset s2 s3)]
+  = admit ()
+
+let lemma_intersect_transitive (s1:subtree_t) (s2:subtree_t)
+  :Lemma (requires True) (ensures (intersect s1 s2 == intersect s2 s1))
+   [SMTPatOr [[SMTPat (intersect s1 s2)]; [SMTPat (intersect s2 s1)]]]
+  = admit ()
+
+let lemma_intersect_union_empty (s1:subtree_t) (s2:subtree_t) (s3:subtree_t)
+  :Lemma (requires (intersect s1 s3 == empty /\ intersect s2 s3 == empty))
+         (ensures  (intersect (union s1 s2) s3 == empty))
+   [SMTPat (intersect (union s1 s2) s3)]
+  = admit ()
+(***** end boring set lemmas *****)
+
 type id (n:nat) = i:nat{i < n}
 
-type elt (n:nat) = id n * id n
+(*
+ * each node maintains its parent id, height, and subtree nodes (including itself)
+ * the subtree set is used as the decreasing metric
+ *)
+type elt (n:nat) = id n * id n * subtree_t
 
 type uf_forest (n:nat) = s:seq (ref (elt n)){length s = n}
 
-(* liveness and separation condition for the forest *)
+(* liveness and separation condition for the unionfind forest *)
 let live (#n:nat) (uf:uf_forest n) (h:heap) :Type0 =
   (forall (i:id n).{:pattern addr_of (index uf i)} forall (j:id n).{:pattern addr_of (index uf j)}
                i <> j ==> addr_of (index uf i) <> addr_of (index uf j)) /\  //all the refs in the forest are distinct
   (forall (i:id n).{:pattern (h `contains_a_well_typed` (index uf i))}
                h `contains_a_well_typed` (index uf i))  //all the refs in the forest are well typed
 
-(* helpers for getting the parent and height *)
-unfold let parent (#n:nat) (uf:uf_forest n) (i:id n) (h:heap) :GTot (id n) = fst (sel h (index uf i))
-unfold let height (#n:nat) (uf:uf_forest n) (i:id n) (h:heap) :GTot (id n) = snd (sel h (index uf i))
+(* helpers for getting the parent, height, and the subtree *)
+unfold let parent  (#n:nat) (uf:uf_forest n) (i:id n) (h:heap) :GTot (id n)    = Mktuple3?._1 (sel h (index uf i))
+unfold let height  (#n:nat) (uf:uf_forest n) (i:id n) (h:heap) :GTot (id n)    = Mktuple3?._2 (sel h (index uf i))
+unfold let subtree (#n:nat) (uf:uf_forest n) (i:id n) (h:heap) :GTot subtree_t = Mktuple3?._3 (sel h (index uf i))
 
 (*
  * well-formed conditions on the forest, essentially the invariants needed for proving the termination of operations
- * TODO: add the pattern, perhaps {:pattern (sel h (index uf i))}?
+ * my suspicion is that these patterns are not too helpful
  *)
 let well_formed (#n:nat) (uf:uf_forest n) (h:heap) =
-  forall (i:id n).{:pattern (sel h (index uf i))}
-             (parent uf i h = i \/ height uf i h < height uf (parent uf i h) h)
+  forall (i:id n). {:pattern (sel h (index uf i))}
+             (let p = parent uf i h in
+	      let s = subtree uf i h in
+	      mem i s /\  //at least i itself is in the subtree
+	      subset s (set_n n) /\  //s is a subset of set_n
+	      (forall (j:id n). {:pattern (sel h (index uf j))}  //different roots have disjoint subtrees
+	                  (i <> j /\ i = p /\ j = parent uf j h) ==> intersect s (subtree uf j h) == empty) /\
+	      (p = i \/ strict_subset s (subtree uf p h)))  //either i is its own parent or subtree of i is a strict subset of subtree of p
+
+(* the metric that decreases in the recursive calls *)
+let diff (n:nat) (s:subtree_t) :Tot nat = size (minus (set_n n) s)
 
 (*
  * the postcondition parent uf r h1 = r is added because of merge, see below in comments
  *)
 reifiable let rec find (#n:nat) (uf:uf_forest n) (i:id n) (ghost_heap:heap)
   :ST (id n) (requires  (fun h0      -> ghost_heap == h0 /\ live uf h0 /\ well_formed uf h0))
-              (ensures   (fun h0 r h1 -> h0 == h1 /\ parent uf r h1 = r))
-	      (decreases (length uf - height #n uf i ghost_heap))
-  = let (p, _) = read (index uf i) in
+             (ensures   (fun h0 r h1 -> h0 == h1 /\ parent uf r h1 = r))
+	     (decreases (diff n (subtree #n uf i ghost_heap)))
+  = let (p, _, _) = read (index uf i) in
     if p = i then i
-    else begin
-      find uf p ghost_heap
-    end      
+    else find uf p ghost_heap
 
-reifiable let rec merge (#n:nat) (uf:uf_forest n) (i_1:id n) (i_2:id n)
-  : ST unit (requires (fun h0      -> live uf h0 /\ well_formed uf h0))
-            (ensures  (fun h0 _ h1 -> live uf h1 /\ well_formed uf h1))
-  = let h0 = STATE?.get () in
+#set-options "--z3rlimit 10"
+let lemma_find_helper (#n:nat) (uf:uf_forest n) (i:id n) (h:heap{live uf h /\ well_formed uf h})
+  :Lemma (let p, _, _ = sel h (index uf i) in
+          reify (find uf p h) h == reify (find uf i h) h)
+  = ()
+#reset-options
 
-    let r_1 = find uf i_1 (STATE?.get ()) in
-    let r_2 = find uf i_2 (STATE?.get ()) in
-
-    let ref_1 = index uf r_1 in
-    let ref_2 = index uf r_2 in
-
-    let _, d_1 = !ref_1 in
-    let _, d_2 = !ref_2 in
-
-    assume (d_1 + 1 < length uf);
-
-    if r_1 = r_2 then ()
-    else begin
-      write ref_1 (r_2, d_1);
-      if d_1 + 1 > d_2 then
-        //after this write, in order to establish the third clause of well_formed,
-	//we need to reason that height of r2's parent is more than d1 + 1, or that r2's parent is r2 itself
-	//but we obtained r2 by calling find, so the clause parent uf r h1 = r, is added so that this can go through
-        write ref_2 (r_2, d_1 + 1)
-    end
-
+#set-options "--z3rlimit 30"
 reifiable let rec find_opt (#n:nat) (uf:uf_forest n) (i:id n) (ghost_heap:heap)
   :ST (id n) (requires (fun h0      -> ghost_heap == h0 /\ live uf h0 /\ well_formed uf h0))
              (ensures  (fun h0 r h1 -> live uf h1 /\ well_formed uf h1 /\ parent uf r h1 = r /\  //these are from find
-	                            (r = i \/ height uf r h1 > height uf i h1) /\  //we need this because when we write p' as i's parent
-				                                                   //we need to ensure wellformedness i.e. height of p'
-										   //is more than the height of i
-				     (forall (j:id n).{:pattern (sel h1 (index uf j))} height uf j h0 < height uf i h0 ==>
-	                                          sel h1 (index uf j) = sel h0 (index uf j))))  //this last clause to say that i remains unchanged in the recursive call, else when we write its height to be d, we have trouble proving that p's height is more than d
-	      (decreases (length uf - height #n uf i ghost_heap))
-  = let (p, d) = read (index uf i) in
+	                            (r = i \/ strict_subset (subtree uf i h1) (subtree uf r h1)) /\  //we need this because when we write p' as i's parent
+				                                                   //we need to ensure wellformedness i.e. subtree of p'
+										   //is a strict superset of subtee of i
+				     (forall (j:id n).{:pattern (sel h1 (index uf j))} strict_subset (subtree uf j h0) (subtree uf i h0) ==>
+	                                          sel h1 (index uf j) = sel h0 (index uf j))))  //this last clause to say that i remains unchanged in the recursive call, else when we write its subtree to be s, we have trouble proving that p's subtree is a strict superset of s
+	      (decreases (diff n (subtree #n uf i ghost_heap)))
+  = let (p, d, s) = read (index uf i) in
     if p = i then i
     else
       let h = STATE?.get () in
       let p' = find_opt uf p h in
-      write (index uf i) (p', d);
+      write (index uf i) (p', d, s);
       p'
-
-#set-options "--z3rlimit 50"
-let lemma_find_helper (#n:nat) (uf:uf_forest n) (i:id n) (h:heap{live uf h /\ well_formed uf h})
-  :Lemma (let p, d = sel h (index uf i) in
-          reify (find uf p h) h == reify (find uf i h) h)
-  = let p, s = sel h (index uf i) in
-    if p = i then ()
-    else ()
 #reset-options
 
+(*
+ * lemma to condense find_opt behavior
+ *)
 #set-options "--z3rlimit 50"
 let lemma_find_opt_helper (#n:nat) (uf:uf_forest n) (i:id n) (h:heap{live uf h /\ well_formed uf h})
-  :Lemma (let p, d = sel h (index uf i) in
+  :Lemma (let p, d, s = sel h (index uf i) in
           p = i \/
 	  (let pp, hp = reify (find_opt uf p h) h in
-            let pi, hi = reify (find_opt uf i h) h in
-	    pp = pi /\ (hi == upd hp (index uf i) (pp, d))))
-  = let p, s = sel h (index uf i) in
+           let pi, hi = reify (find_opt uf i h) h in
+	   pp = pi /\ (hi == upd hp (index uf i) (pp, d, s))))
+  = let p, s, _ = sel h (index uf i) in
     if p = i then ()
-    else ()
+    else begin
+      ignore (reify (find_opt uf p h) h);
+      ignore (reify (find_opt uf i h) h);
+      ()
+    end
 #reset-options
 
-(* let lemma_0 (uf:uf_forest) (i:id uf) (h:heap{live uf h /\ well_formed uf h}) :GTot unit = *)
-(*   let p, s = sel h (index uf i) in *)
-(*   if p = i then () *)
-(*   else begin *)
-(*     let pp, h1 = reify (find_opt uf p h) h in *)
-(*     let _, h2 = reify (find_opt uf i h) h in *)
-(*     assert (h2 == upd h1 (index uf i) (pp, s)); *)
-(*     () *)
-(*   end *)
-
-(* let lemma_1 (uf:uf_forest) (i:id uf) (h:heap{live uf h /\ well_formed uf h}) :GTot unit = *)
-(*   let p, s = sel h (index uf i) in *)
-(*   if p = i then () *)
-(*   else begin *)
-(*     let pp, h1 = reify (find_opt uf p h) h in *)
-(*     let _, h2 = reify (find_opt uf i h) h in *)
-(*     assert (forall (a:Type) (r:ref a). addr_of r <> addr_of (index uf i) ==> sel h1 r == sel h2 r); *)
-(*     //assert (h2 == upd h1 (index uf i) (pp, s)); *)
-(*     () *)
-(*   end *)
 (*
  * a simple warm up lemma
  * proving that find and find_opt return the same value
@@ -134,8 +163,8 @@ let lemma_find_opt_helper (#n:nat) (uf:uf_forest n) (i:id n) (h:heap{live uf h /
 let rec lemma_find_find_opt_same_result (#n:nat) (uf:uf_forest n) (i:id n) (h:heap{live uf h /\ well_formed uf h})
   :Lemma (requires  True)
          (ensures   (fst (reify (find uf i h) h) = fst (reify (find_opt uf i h) h)))
-	 (decreases (length uf - height #n uf i h))
-  = let p, _ = sel h (index uf i) in
+	 (decreases (diff n (subtree #n uf i h)))
+  = let p, _, _ = sel h (index uf i) in
     if p = i then ()
     else begin
       lemma_find_find_opt_same_result uf p h
@@ -154,8 +183,8 @@ let rec lemma_find_opt_parent_same_as_find_root (#n:nat) (uf:uf_forest n) (i:id 
 		    let p1 = parent uf j h1 in
 
                     p0 = p1 \/ (p1 = fst (reify (find uf j h0) h0) /\ parent uf p1 h1 = p1)))
-	 (decreases (length uf - height #n uf i h))
-  = let p, _ = sel h (index uf i) in
+	 (decreases (diff n (subtree #n uf i h)))
+  = let p, _, _ = sel h (index uf i) in
     if p = i then ()
     else begin
       lemma_find_opt_parent_same_as_find_root uf p h j;
@@ -175,7 +204,7 @@ let rec lemma_find_opt_parent_same_as_find_root (#n:nat) (uf:uf_forest n) (i:id 
  * in particular, we prove that find of a node j in h1 (the resultant heap after path compression)
  * is same as find of j in h0
  *)
-#set-options "--z3rlimit 50"
+#set-options "--z3rlimit 100"
 let rec lemma_find_find_opt_equivalence (#n:nat) (uf:uf_forest n) (i:id n) (h:heap{live uf h /\ well_formed uf h}) (j:id n)
   :Lemma (requires True)
          (ensures  (let _, h0 = reify (find uf i h) h in
@@ -184,21 +213,23 @@ let rec lemma_find_find_opt_equivalence (#n:nat) (uf:uf_forest n) (i:id n) (h:he
                     let r0, _ = reify (find uf j h0) h0 in
 		    let r1, _ = reify (find uf j h1) h1 in
 		    r0 = r1))  //root of a node remains same in h0 and h1, i.e. find_opt does not change the find query
-	 (decreases (length uf - height #n uf j h))
+	 (decreases (diff n (subtree #n uf j h)))
   = 
     let _, h0 = reify (find uf i h) h in
     let _, h1 = reify (find_opt uf i h) h in
 
     lemma_find_opt_parent_same_as_find_root uf i h j;
 
-    let p0, _ = sel h0 (index uf j) in
-    let p1, _ = sel h1 (index uf j) in
+    let p0, _, _ = sel h0 (index uf j) in
+    let p1, _, _ = sel h1 (index uf j) in
     lemma_find_helper uf j h0;
     lemma_find_helper uf j h1;
+    assert (reify (find uf j h0) h0 == reify (find uf p0 h0) h0);
+    assert (reify (find uf j h1) h1 == reify (find uf p1 h1) h1);
 
     //lemma_find_opt_parent_same_as_find_root tells us that either p0 = p1,
     //or p1 = root of j in h0
-  
+    assert (p0 = p1 \/ (p1 = fst (reify (find uf j h0) h0) /\ parent uf p1 h1 = p1));
     if p0 = p1 then begin
       if j = p0 then ()  //if j = p0 = p1, then find returns j immediately, so we are done
       else begin  //else we invoke I.H. on p0, and then one unrolling of find call on j uses it to give us the proof
@@ -210,5 +241,28 @@ let rec lemma_find_find_opt_equivalence (#n:nat) (uf:uf_forest n) (i:id n) (h:he
         assert (p1 = fst (reify (find uf j h0) h0));
 	assert (parent uf p1 h1 = p1);
 	assert (p1 = fst (reify (find uf p1 h1) h1));
+	assert (fst (reify (find uf j h1) h1) = fst (reify (find uf p1 h1) h1));
 	()
       end
+#reset-options
+
+reifiable let rec merge (#n:nat) (uf:uf_forest n) (i_1:id n) (i_2:id n)
+  : ST unit (requires (fun h0      -> live uf h0 /\ well_formed uf h0))
+            (ensures  (fun h0 _ h1 -> live uf h1 /\ well_formed uf h1))
+  = let h0 = STATE?.get () in
+
+    let r_1 = find uf i_1 (STATE?.get ()) in
+    let r_2 = find uf i_2 (STATE?.get ()) in
+
+    let ref_1 = index uf r_1 in
+    let ref_2 = index uf r_2 in
+
+    let _, d_1, s_1 = !ref_1 in
+    let _, d_2, s_2 = !ref_2 in
+
+    if r_1 = r_2 then ()
+    else begin
+      write ref_1 (r_2, d_1, s_1);
+      write ref_2 (r_2, d_2, union s_1 s_2);
+      assert (strict_subset s_1 (union s_1 s_2))
+    end
